theories/Labelled_Transition_System/Examples_of_LTS/VCCS/Testing/VCCS_ta_tc_gen.v
@@ -134,16 +134,27 @@ destruct p; intros.
 Qed.
 
 
-Lemma Eval_simpl_true v : Eval_Eq (v == v) = Some true <-> v = v.
+Lemma Eval_simpl_true n v : Eval_Eq n (v == v) = Some true <-> v = v.
 Proof.
   split.
   - intro e. inversion e. destruct v; rewrite decide_True in H0; eauto.
   - intro e. subst. simpl. destruct v; rewrite decide_True; eauto.
 Qed.
 
-Lemma Eval_simpl_false v1 v2 : v1 ≠ v2 ->  Eval_Eq (cst v1 == cst v2) = Some false.
+Lemma Eval_simpl_false n v1 v2 : v1 ≠ v2 ->  Eval_Eq n (cst v1 == cst v2) = Some false.
 Proof.
   - intro e. simpl. rewrite decide_False; eauto.
+Qed.
+
+Lemma Eval_simpl_false_gen (v1 v2 : ValueData) : v1 ≠ v2 -> Eval_Eq 0 (v1 == v2) = Some false.
+Proof.
+  intros neq. destruct v1 as [t1|i1], v2 as [t2|i2]; simpl.
+  - destruct (decide (t1 = t2)) as [->|]. contradiction (neq eq_refl). reflexivity.
+  - reflexivity.
+  - reflexivity.
+  - destruct (decide (i1 = i2)) as [->|].
+    + contradiction (neq eq_refl).
+    + reflexivity.
 Qed.
 
 Lemma New_Var_And_NewVar_in_Data : forall j i e, NewVar_in_Data (i + S j) (NewVar_in_Data i e) = NewVar_in_Data i (NewVar_in_Data (i + j) e).
@@ -374,29 +385,22 @@ Inductive Well_Defined_Trace : trace (ExtAct TypeOfActions) -> Prop :=
                                                     -> Well_Defined_Trace (a :: s).
 
 Lemma gen_test_gen_spec_good_not_mu e μ  μ' s p :
-  Well_Defined_ExtAction (μ)
-  -> Well_Defined_ExtAction (μ') 
-    -> lts (gen_test (μ  :: s) p) (ActExt $ μ') e -> μ' ≠ μ -> good_VCCS e.
+  lts (gen_test (μ  :: s) p) (ActExt $ μ') e -> μ' ≠ μ -> good_VCCS e.
 Proof.
-  intros WD_trace WD_action tr neq. unfold gen_test in tr. simpl in *. 
+  intros tr neq. unfold gen_test in tr. simpl in *.
   destruct μ; destruct a; subst. inversion tr;subst.
-  + inversion WD_trace; subst.
-    inversion WD_action; subst.
-    ++ simpl in *. inversion tr; subst.
-       +++ inversion H4.
-       +++ inversion H4.
-    ++ inversion tr; subst.
-       +++ inversion H3. subst.
-           simpl in *. assert (v ≠ v0) as neq'. 
-           { intro. subst. contradiction. }
-           eapply Eval_simpl_false in neq'.
-           assert ((If cst v == cst v0
-                      Then gen_test_raw (NewVar_in_trace 0 s) s (NewVar 0 p) ^ (cst v0)
-                      Else ①) ≡ ①).
-           { eapply cgr_if_false_step; eauto. }
-           eapply good_preserved_by_cgr_step; eauto. eapply good_success.
-           eapply cgr_if_false_rev_step; eauto.
-       +++ subst. inversion H4.
+  + simpl in *. inversion tr; subst.
+    - inversion H3. subst. simpl in *. rewrite All_AccordingTo_Data in *.
+      assert (v0 ≠ v) as neq'.
+      { intro. subst. contradiction. }
+      eapply Eval_simpl_false_gen in neq'.
+      assert ((If v0 == v
+                 Then gen_test_raw (NewVar_in_trace 0 s) s (NewVar 0 p) ^ v0
+                 Else ①) ≡ ①).
+      { eapply cgr_if_false_step; eauto. }
+      eapply good_preserved_by_cgr_step; eauto. eapply good_success.
+      eapply cgr_if_false_rev_step; eauto.
+    - subst. inversion H4.
   + inversion H3.
   + inversion tr.
     - subst. inversion H3. subst. exfalso. eapply neq. eauto.
@@ -411,8 +415,6 @@ Fixpoint unroll_fw (L : list PreAct) : gproc :=
   end.
 
 Definition gen_acc (G : gset PreAct) s := gen_test s (g (unroll_fw (elements G))).
-
-Parameter Hyp_WD_acc : forall α s e G, lts (gen_acc G s) α e -> Well_Defined_Trace s /\ Well_Defined_Action α.
 
 Lemma unroll_a_eq_perm (xs ys : list PreAct) : xs ≡ₚ ys -> (g (unroll_fw xs)) ≡* (g (unroll_fw ys)).
 Proof.
@@ -472,15 +474,7 @@ Next Obligation.
 Qed.
 Next Obligation.
   intros g t'. intros.
-  simpl in *. assert (lts (gen_acc g (β :: s)) (ActExt μ) t') as Hyp_tr; eauto.
-  eapply Hyp_WD_acc in Hyp_tr as (WD_trace & WD_action) ; eauto.
-  assert (Well_Defined_ExtAction β) as Hyp.
-  { inversion WD_trace. subst; eauto. }
-  assert (Well_Defined_ExtAction μ) as Hyp'.
-  { inversion WD_action; subst; eauto.
-    + constructor.
-    + constructor. }
-  eapply gen_test_gen_spec_good_not_mu. exact Hyp. exact Hyp'. eauto. eauto.
+  simpl in *. eapply gen_test_gen_spec_good_not_mu; eauto.
 Qed.
 
 Lemma gen_acc_does_not_tau : forall g r, ~ lts (unroll_fw g) τ r.
@@ -668,7 +662,6 @@ Next Obligation.
 Qed.
 
 Definition gen_conv s := gen_test s (𝛕 • ①).
-Parameter Hyp_WD_conv : forall α s e, lts (gen_conv s) α e -> Well_Defined_Trace s /\ Well_Defined_Action α.
 
 #[global] Program Instance gen_conv_gen_test_inst
 : test_spec gen_conv.
@@ -690,15 +683,7 @@ Next Obligation.
 Qed.
 Next Obligation.
   intros t'. intros.
-  simpl in *. assert (lts (gen_conv (β :: s)) (ActExt μ) t') as Hyp_tr; eauto.
-  eapply Hyp_WD_conv in Hyp_tr as (WD_trace & WD_action) ; eauto.
-  assert (Well_Defined_ExtAction β) as Hyp.
-  { inversion WD_trace. subst; eauto. }
-  assert (Well_Defined_ExtAction μ) as Hyp'.
-  { inversion WD_action; subst; eauto.
-    + constructor.
-    + constructor. }
-  eapply gen_test_gen_spec_good_not_mu. exact Hyp. exact Hyp'. eauto. eauto.
+  simpl in *. eapply gen_test_gen_spec_good_not_mu; eauto.
 Qed.
 
 #[global] Program Instance gen_conv_gen_spec_conv_inst
